WIP: fix ELI

src/tlogic/LiveObligations.v
@@ -875,49 +875,72 @@ Section ELI.
   Context `{ARROWSHOTRA : @GRA.inG ArrowShotRA Σ}.
   Context `{ARROWRA : @GRA.inG ArrowRA Σ}.
 
-  Fixpoint env_live_inv (n : nat) {v x : nat} E (k : nat) (P T : Vars v) : iProp :=
+  Fixpoint env_live_inv (n : nat) (x : nat) E (k : nat) {v} (A T : Vars v) : iProp :=
     match n with
-    | O => prop _ T
+    | O => ⌜False⌝%I
     | S m =>
-        □ ((prop _ P ∗ €) =| x |=( fairI (ident_tgt:=ident_tgt) x )={ E }=∗ ((prop _ P ∗ ◇[k](0, 1)) ∨ (∃ (R : Vars v), prop _ R ∗ @env_live_inv m v x E k R T)))%I
+        □(∃ (P : Vars v),
+             (prop _ P)
+               ∗
+               ((prop _ P ∗ €)
+                  -∗ (prop _ A)
+                  =| x |=( fairI (ident_tgt:=ident_tgt) x )={ E }=∗ ((prop _ A ∗ ◇[k](0, 1)) ∨ (prop _ A ∗ @env_live_inv m x E k v A T) ∨ (prop _ T))))%I
     end.
 
-  Lemma eli_lo_ind k l n v x E (T : Vars v) (Q : iProp) :
-    (v < x) ->
+  Lemma eli_lo_ind k l n x E v (A T : Vars v) (Q : iProp) :
+    (v <= x) ->
     (◆[k, l])
-      ⊢ (□((€ =|x|=(fairI (ident_tgt:=ident_tgt) x)={E}=∗ Q) =|x|=(fairI (ident_tgt:=ident_tgt) x)={E}=∗ Q))
+      ⊢
+      (□((€ -∗ (prop _ A) =|x|=(fairI (ident_tgt:=ident_tgt) x)={E}=∗ Q) -∗ (prop _ A) =|x|=(fairI (ident_tgt:=ident_tgt) x)={E}=∗ Q))
       -∗
-      (prop _ T -∗ Q)
+      ((prop _ T) =|x|=(fairI (ident_tgt:=ident_tgt) x)={E}=∗ Q)
       -∗
-      (∀ (P : Vars v), (prop _ P) -∗ (@env_live_inv n v x E k P T)  =|x|=(fairI (ident_tgt:=ident_tgt) x)={E}=∗ Q)
-      (* (∀ (P : Vars v), (prop _ P) -∗ (@env_live_inv n v x E k P T) -∗ (prop _ P -∗ prop _ T -∗ Q) =|x|=(fairI (ident_tgt:=ident_tgt) x)={E}=∗ Q) *)
+      ((prop _ A ∗ @env_live_inv n x E k v A T) =|x|=(fairI (ident_tgt:=ident_tgt) x)={E}=∗ Q)
   .
   Proof.
     (* Outer induction. *)
     iIntros (LT). pattern n. induction n.
-    { iIntros "_ #IH TERM %P PP ELI". ss. iModIntro. iApply ("TERM" with "ELI"). }
-    (* iIntros "(%c & %o & #LO) #IH %P TERM PP ELI". *)
+    { iIntros "_ _ TERM [_ F]". ss. }
     iIntros "(%c & %o & #LO)".
     (* Inner induction. *)
     iStopProof. pattern o. revert o. apply (well_founded_ind Ord.lt_well_founded). intros o IHo.
-    iIntros "#LO #IH TERM %P PP ELI". iEval (simpl) in "ELI". iPoseProof "ELI" as "#ELI".
-    iApply "IH". iIntros "FC".
-    iMod ("ELI" with "[PP FC]") as "[(PP & PCk) | (%R & PR & ELI2)]".
-    iFrame.
+    iIntros "#LO #IH TERM [AP ELI]".
+    iEval (simpl) in "ELI". iPoseProof "ELI" as "(%P & #PP & #ELI)".
+    iApply ("IH" with "[TERM] AP"). iIntros "FC AP".
+    iMod ("ELI" with "[FC] AP") as "[(PA & PCk) | [(PA & ELI2) | PT]]".
+    { iFrame. eauto. }
     { (* Prove with the inner induction. *)
       iMod (lo_pc_decr with "[PCk]") as "(%o' & #LO' & %LTo)".
       2:{ iSplitR; iFrame. eauto. }
       lia.
       specialize (IHo o' LTo).
-      iPoseProof (IHo with "LO' IH TERM") as "IHo". iSpecialize ("IHo" $! P with "PP ELI").
-      iFrame.
+      iApply (IHo with "LO' IH TERM [-]"). iFrame. iEval simpl.
+      iModIntro. iExists P. iSplitL; eauto.
     }
     { (* Prove with the outer induction. *)
       iPoseProof (IHn with "[] IH TERM") as "IHn".
       { iExists _, _. eauto. }
-      iSpecialize ("IHn" $! R with "PR ELI2").
-      iFrame.
+      iSpecialize ("IHn" with "[PA ELI2]").
+      iFrame. iFrame.
     }
+    { (* Reached the target state T. *)
+      iApply ("TERM" with "PT").
+    }
+  Qed.
+
+  Lemma ELI_persistent n x E k v (A T : Vars v) :
+    (Persistent (prop _ T)) -> (@env_live_inv n x E k v A T) -∗ □(@env_live_inv n x E k v A T).
+  Proof.
+    iIntros (PERST). pattern n. induction n.
+    { simpl. iIntros "#PT". eauto. }
+    simpl. iIntros "#ELI". eauto.
+  Qed.
+
+  Global Program Instance Persistent_ELI n x E k v (A T : Vars v)
+         (T_PERS : Persistent (prop _ T)) :
+    Persistent (@env_live_inv n x E k v A T).
+  Next Obligation.
+    iIntros "ELI". iPoseProof (ELI_persistent with "ELI") as "ELI". auto.
   Qed.
 
 End ELI.
